Simple formalization of condition variables.

progs/cond.c
@@ -1,0 +1,45 @@
+#include "threads.h"
+//#include <stdio.h>
+#include <stdlib.h>
+
+lock_t mutex, tlock;
+cond_t cond;
+int data[1];
+
+void thread_func(void *args) {
+  lock_t *l = &mutex;
+  lock_t *t = &tlock;
+  cond_t *c = &cond;
+  acquire(l);
+  data[0] = 1;
+  signal(c);
+  release(l);
+  release2(t);
+  return;
+}
+
+int main(void)
+{
+  data[0] = 0;
+  lock_t *l = &mutex;
+  lock_t *t = &tlock;
+  cond_t *c = &cond;
+  makecond(c);
+  makelock(l);
+  makelock(t);
+  spawn_thread((void *)&thread_func, (void *)NULL);
+
+  int v = 0;
+  while(!v){
+    wait(c, l);
+    v = data[0];
+  }
+
+  acquire(t);
+  freelock2(t);
+  freelock(l);
+  freecond(c);
+
+  //  printf("I'm done with a final counter of: %d\n", v);
+  return v;
+}
