progs/threads.h
@@ -3,6 +3,8 @@
 /* typedef struct {char a[8]; void* b[4];} lock_t; */
 typedef struct lock_t {char a[8]; void* b[6];} lock_t;
 
+typedef int cond_t;
+
 void makelock(lock_t *lock);
 
 void freelock(lock_t *lock);
@@ -18,3 +20,13 @@ void release2(lock_t *lock); //consumes the lock
 void spawn_thread(void* (*f)(void*), void* args);
 
 void exit_thread(void);
+
+void makecond(cond_t *cond);
+
+void freecond(cond_t *cond);
+
+void wait(cond_t *cond, lock_t *mutex);
+//for some reason, Pthreads only requires a mutex for wait
+
+void signal(cond_t *cond);
+//unlocks any mutex associated with an active wait call
