progs/cond.v
@@ -1,0 +1,582 @@
+
+Require Import Clightdefs.
+Local Open Scope Z_scope.
+Definition ___builtin_annot : ident := 6%positive.
+Definition ___builtin_annot_intval : ident := 7%positive.
+Definition ___builtin_bswap : ident := 30%positive.
+Definition ___builtin_bswap16 : ident := 32%positive.
+Definition ___builtin_bswap32 : ident := 31%positive.
+Definition ___builtin_clz : ident := 33%positive.
+Definition ___builtin_clzl : ident := 34%positive.
+Definition ___builtin_clzll : ident := 35%positive.
+Definition ___builtin_ctz : ident := 36%positive.
+Definition ___builtin_ctzl : ident := 37%positive.
+Definition ___builtin_ctzll : ident := 38%positive.
+Definition ___builtin_debug : ident := 51%positive.
+Definition ___builtin_fabs : ident := 4%positive.
+Definition ___builtin_fmadd : ident := 42%positive.
+Definition ___builtin_fmax : ident := 40%positive.
+Definition ___builtin_fmin : ident := 41%positive.
+Definition ___builtin_fmsub : ident := 43%positive.
+Definition ___builtin_fnmadd : ident := 44%positive.
+Definition ___builtin_fnmsub : ident := 45%positive.
+Definition ___builtin_fsqrt : ident := 39%positive.
+Definition ___builtin_membar : ident := 8%positive.
+Definition ___builtin_memcpy_aligned : ident := 5%positive.
+Definition ___builtin_nop : ident := 50%positive.
+Definition ___builtin_read16_reversed : ident := 46%positive.
+Definition ___builtin_read32_reversed : ident := 47%positive.
+Definition ___builtin_va_arg : ident := 10%positive.
+Definition ___builtin_va_copy : ident := 11%positive.
+Definition ___builtin_va_end : ident := 12%positive.
+Definition ___builtin_va_start : ident := 9%positive.
+Definition ___builtin_write16_reversed : ident := 48%positive.
+Definition ___builtin_write32_reversed : ident := 49%positive.
+Definition ___compcert_va_composite : ident := 16%positive.
+Definition ___compcert_va_float64 : ident := 15%positive.
+Definition ___compcert_va_int32 : ident := 13%positive.
+Definition ___compcert_va_int64 : ident := 14%positive.
+Definition ___i64_dtos : ident := 17%positive.
+Definition ___i64_dtou : ident := 18%positive.
+Definition ___i64_sar : ident := 29%positive.
+Definition ___i64_sdiv : ident := 23%positive.
+Definition ___i64_shl : ident := 27%positive.
+Definition ___i64_shr : ident := 28%positive.
+Definition ___i64_smod : ident := 25%positive.
+Definition ___i64_stod : ident := 19%positive.
+Definition ___i64_stof : ident := 21%positive.
+Definition ___i64_udiv : ident := 24%positive.
+Definition ___i64_umod : ident := 26%positive.
+Definition ___i64_utod : ident := 20%positive.
+Definition ___i64_utof : ident := 22%positive.
+Definition _a : ident := 1%positive.
+Definition _acquire : ident := 55%positive.
+Definition _args : ident := 67%positive.
+Definition _b : ident := 2%positive.
+Definition _c : ident := 70%positive.
+Definition _cond : ident := 65%positive.
+Definition _data : ident := 66%positive.
+Definition _freecond : ident := 60%positive.
+Definition _freelock : ident := 53%positive.
+Definition _freelock2 : ident := 54%positive.
+Definition _l : ident := 68%positive.
+Definition _lock_t : ident := 3%positive.
+Definition _main : ident := 73%positive.
+Definition _makecond : ident := 59%positive.
+Definition _makelock : ident := 52%positive.
+Definition _mutex : ident := 63%positive.
+Definition _release : ident := 56%positive.
+Definition _release2 : ident := 57%positive.
+Definition _signal : ident := 62%positive.
+Definition _spawn_thread : ident := 58%positive.
+Definition _t : ident := 69%positive.
+Definition _thread_func : ident := 71%positive.
+Definition _tlock : ident := 64%positive.
+Definition _v : ident := 72%positive.
+Definition _wait : ident := 61%positive.
+
+Definition v_mutex := {|
+  gvar_info := (Tstruct _lock_t noattr);
+  gvar_init := (Init_space 32 :: nil);
+  gvar_readonly := false;
+  gvar_volatile := false
+|}.
+
+Definition v_tlock := {|
+  gvar_info := (Tstruct _lock_t noattr);
+  gvar_init := (Init_space 32 :: nil);
+  gvar_readonly := false;
+  gvar_volatile := false
+|}.
+
+Definition v_cond := {|
+  gvar_info := tint;
+  gvar_init := (Init_space 4 :: nil);
+  gvar_readonly := false;
+  gvar_volatile := false
+|}.
+
+Definition v_data := {|
+  gvar_info := (tarray tint 1);
+  gvar_init := (Init_space 4 :: nil);
+  gvar_readonly := false;
+  gvar_volatile := false
+|}.
+
+Definition f_thread_func := {|
+  fn_return := tvoid;
+  fn_callconv := cc_default;
+  fn_params := ((_args, (tptr tvoid)) :: nil);
+  fn_vars := nil;
+  fn_temps := ((_l, (tptr (Tstruct _lock_t noattr))) ::
+               (_t, (tptr (Tstruct _lock_t noattr))) :: (_c, (tptr tint)) ::
+               nil);
+  fn_body :=
+(Ssequence
+  (Sset _l
+    (Eaddrof (Evar _mutex (Tstruct _lock_t noattr))
+      (tptr (Tstruct _lock_t noattr))))
+  (Ssequence
+    (Sset _t
+      (Eaddrof (Evar _tlock (Tstruct _lock_t noattr))
+        (tptr (Tstruct _lock_t noattr))))
+    (Ssequence
+      (Sset _c (Eaddrof (Evar _cond tint) (tptr tint)))
+      (Ssequence
+        (Scall None
+          (Evar _acquire (Tfunction
+                           (Tcons (tptr (Tstruct _lock_t noattr)) Tnil) tvoid
+                           cc_default))
+          ((Etempvar _l (tptr (Tstruct _lock_t noattr))) :: nil))
+        (Ssequence
+          (Sassign
+            (Ederef
+              (Ebinop Oadd (Evar _data (tarray tint 1))
+                (Econst_int (Int.repr 0) tint) (tptr tint)) tint)
+            (Econst_int (Int.repr 1) tint))
+          (Ssequence
+            (Scall None
+              (Evar _signal (Tfunction (Tcons (tptr tint) Tnil) tvoid
+                              cc_default))
+              ((Etempvar _c (tptr tint)) :: nil))
+            (Ssequence
+              (Scall None
+                (Evar _release (Tfunction
+                                 (Tcons (tptr (Tstruct _lock_t noattr)) Tnil)
+                                 tvoid cc_default))
+                ((Etempvar _l (tptr (Tstruct _lock_t noattr))) :: nil))
+              (Ssequence
+                (Scall None
+                  (Evar _release2 (Tfunction
+                                    (Tcons (tptr (Tstruct _lock_t noattr))
+                                      Tnil) tvoid cc_default))
+                  ((Etempvar _t (tptr (Tstruct _lock_t noattr))) :: nil))
+                (Sreturn None)))))))))
+|}.
+
+Definition f_main := {|
+  fn_return := tint;
+  fn_callconv := cc_default;
+  fn_params := nil;
+  fn_vars := nil;
+  fn_temps := ((_l, (tptr (Tstruct _lock_t noattr))) ::
+               (_t, (tptr (Tstruct _lock_t noattr))) :: (_c, (tptr tint)) ::
+               (_v, tint) :: nil);
+  fn_body :=
+(Ssequence
+  (Ssequence
+    (Sassign
+      (Ederef
+        (Ebinop Oadd (Evar _data (tarray tint 1))
+          (Econst_int (Int.repr 0) tint) (tptr tint)) tint)
+      (Econst_int (Int.repr 0) tint))
+    (Ssequence
+      (Sset _l
+        (Eaddrof (Evar _mutex (Tstruct _lock_t noattr))
+          (tptr (Tstruct _lock_t noattr))))
+      (Ssequence
+        (Sset _t
+          (Eaddrof (Evar _tlock (Tstruct _lock_t noattr))
+            (tptr (Tstruct _lock_t noattr))))
+        (Ssequence
+          (Sset _c (Eaddrof (Evar _cond tint) (tptr tint)))
+          (Ssequence
+            (Scall None
+              (Evar _makecond (Tfunction (Tcons (tptr tint) Tnil) tvoid
+                                cc_default))
+              ((Etempvar _c (tptr tint)) :: nil))
+            (Ssequence
+              (Scall None
+                (Evar _makelock (Tfunction
+                                  (Tcons (tptr (Tstruct _lock_t noattr))
+                                    Tnil) tvoid cc_default))
+                ((Etempvar _l (tptr (Tstruct _lock_t noattr))) :: nil))
+              (Ssequence
+                (Scall None
+                  (Evar _makelock (Tfunction
+                                    (Tcons (tptr (Tstruct _lock_t noattr))
+                                      Tnil) tvoid cc_default))
+                  ((Etempvar _t (tptr (Tstruct _lock_t noattr))) :: nil))
+                (Ssequence
+                  (Scall None
+                    (Evar _spawn_thread (Tfunction
+                                          (Tcons
+                                            (tptr (Tfunction
+                                                    (Tcons (tptr tvoid) Tnil)
+                                                    (tptr tvoid) cc_default))
+                                            (Tcons (tptr tvoid) Tnil)) tvoid
+                                          cc_default))
+                    ((Ecast
+                       (Eaddrof
+                         (Evar _thread_func (Tfunction
+                                              (Tcons (tptr tvoid) Tnil) tvoid
+                                              cc_default))
+                         (tptr (Tfunction (Tcons (tptr tvoid) Tnil) tvoid
+                                 cc_default))) (tptr tvoid)) ::
+                     (Ecast (Econst_int (Int.repr 0) tint) (tptr tvoid)) ::
+                     nil))
+                  (Ssequence
+                    (Sset _v (Econst_int (Int.repr 0) tint))
+                    (Ssequence
+                      (Swhile
+                        (Eunop Onotbool (Etempvar _v tint) tint)
+                        (Ssequence
+                          (Scall None
+                            (Evar _wait (Tfunction
+                                          (Tcons (tptr tint)
+                                            (Tcons
+                                              (tptr (Tstruct _lock_t noattr))
+                                              Tnil)) tvoid cc_default))
+                            ((Etempvar _c (tptr tint)) ::
+                             (Etempvar _l (tptr (Tstruct _lock_t noattr))) ::
+                             nil))
+                          (Sset _v
+                            (Ederef
+                              (Ebinop Oadd (Evar _data (tarray tint 1))
+                                (Econst_int (Int.repr 0) tint) (tptr tint))
+                              tint))))
+                      (Ssequence
+                        (Scall None
+                          (Evar _acquire (Tfunction
+                                           (Tcons
+                                             (tptr (Tstruct _lock_t noattr))
+                                             Tnil) tvoid cc_default))
+                          ((Etempvar _t (tptr (Tstruct _lock_t noattr))) ::
+                           nil))
+                        (Ssequence
+                          (Scall None
+                            (Evar _freelock2 (Tfunction
+                                               (Tcons
+                                                 (tptr (Tstruct _lock_t noattr))
+                                                 Tnil) tvoid cc_default))
+                            ((Etempvar _t (tptr (Tstruct _lock_t noattr))) ::
+                             nil))
+                          (Ssequence
+                            (Scall None
+                              (Evar _freelock (Tfunction
+                                                (Tcons
+                                                  (tptr (Tstruct _lock_t noattr))
+                                                  Tnil) tvoid cc_default))
+                              ((Etempvar _l (tptr (Tstruct _lock_t noattr))) ::
+                               nil))
+                            (Ssequence
+                              (Scall None
+                                (Evar _freecond (Tfunction
+                                                  (Tcons (tptr tint) Tnil)
+                                                  tvoid cc_default))
+                                ((Etempvar _c (tptr tint)) :: nil))
+                              (Sreturn (Some (Etempvar _v tint)))))))))))))))))
+  (Sreturn (Some (Econst_int (Int.repr 0) tint))))
+|}.
+
+Definition composites : list composite_definition :=
+(Composite _lock_t Struct
+   ((_a, (tarray tschar 8)) :: (_b, (tarray (tptr tvoid) 6)) :: nil)
+   noattr :: nil).
+
+Definition prog : Clight.program := {|
+prog_defs :=
+((___builtin_fabs,
+   Gfun(External (EF_builtin "__builtin_fabs"
+                   (mksignature (AST.Tfloat :: nil) (Some AST.Tfloat)
+                     cc_default)) (Tcons tdouble Tnil) tdouble cc_default)) ::
+ (___builtin_memcpy_aligned,
+   Gfun(External (EF_builtin "__builtin_memcpy_aligned"
+                   (mksignature
+                     (AST.Tint :: AST.Tint :: AST.Tint :: AST.Tint :: nil)
+                     None cc_default))
+     (Tcons (tptr tvoid)
+       (Tcons (tptr tvoid) (Tcons tuint (Tcons tuint Tnil)))) tvoid
+     cc_default)) ::
+ (___builtin_annot,
+   Gfun(External (EF_builtin "__builtin_annot"
+                   (mksignature (AST.Tint :: nil) None
+                     {|cc_vararg:=true; cc_unproto:=false; cc_structret:=false|}))
+     (Tcons (tptr tschar) Tnil) tvoid
+     {|cc_vararg:=true; cc_unproto:=false; cc_structret:=false|})) ::
+ (___builtin_annot_intval,
+   Gfun(External (EF_builtin "__builtin_annot_intval"
+                   (mksignature (AST.Tint :: AST.Tint :: nil) (Some AST.Tint)
+                     cc_default)) (Tcons (tptr tschar) (Tcons tint Tnil))
+     tint cc_default)) ::
+ (___builtin_membar,
+   Gfun(External (EF_builtin "__builtin_membar"
+                   (mksignature nil None cc_default)) Tnil tvoid cc_default)) ::
+ (___builtin_va_start,
+   Gfun(External (EF_builtin "__builtin_va_start"
+                   (mksignature (AST.Tint :: nil) None cc_default))
+     (Tcons (tptr tvoid) Tnil) tvoid cc_default)) ::
+ (___builtin_va_arg,
+   Gfun(External (EF_builtin "__builtin_va_arg"
+                   (mksignature (AST.Tint :: AST.Tint :: nil) None
+                     cc_default)) (Tcons (tptr tvoid) (Tcons tuint Tnil))
+     tvoid cc_default)) ::
+ (___builtin_va_copy,
+   Gfun(External (EF_builtin "__builtin_va_copy"
+                   (mksignature (AST.Tint :: AST.Tint :: nil) None
+                     cc_default))
+     (Tcons (tptr tvoid) (Tcons (tptr tvoid) Tnil)) tvoid cc_default)) ::
+ (___builtin_va_end,
+   Gfun(External (EF_builtin "__builtin_va_end"
+                   (mksignature (AST.Tint :: nil) None cc_default))
+     (Tcons (tptr tvoid) Tnil) tvoid cc_default)) ::
+ (___compcert_va_int32,
+   Gfun(External (EF_external "__compcert_va_int32"
+                   (mksignature (AST.Tint :: nil) (Some AST.Tint) cc_default))
+     (Tcons (tptr tvoid) Tnil) tuint cc_default)) ::
+ (___compcert_va_int64,
+   Gfun(External (EF_external "__compcert_va_int64"
+                   (mksignature (AST.Tint :: nil) (Some AST.Tlong)
+                     cc_default)) (Tcons (tptr tvoid) Tnil) tulong
+     cc_default)) ::
+ (___compcert_va_float64,
+   Gfun(External (EF_external "__compcert_va_float64"
+                   (mksignature (AST.Tint :: nil) (Some AST.Tfloat)
+                     cc_default)) (Tcons (tptr tvoid) Tnil) tdouble
+     cc_default)) ::
+ (___compcert_va_composite,
+   Gfun(External (EF_external "__compcert_va_composite"
+                   (mksignature (AST.Tint :: AST.Tint :: nil) (Some AST.Tint)
+                     cc_default)) (Tcons (tptr tvoid) (Tcons tuint Tnil))
+     (tptr tvoid) cc_default)) ::
+ (___i64_dtos,
+   Gfun(External (EF_runtime "__i64_dtos"
+                   (mksignature (AST.Tfloat :: nil) (Some AST.Tlong)
+                     cc_default)) (Tcons tdouble Tnil) tlong cc_default)) ::
+ (___i64_dtou,
+   Gfun(External (EF_runtime "__i64_dtou"
+                   (mksignature (AST.Tfloat :: nil) (Some AST.Tlong)
+                     cc_default)) (Tcons tdouble Tnil) tulong cc_default)) ::
+ (___i64_stod,
+   Gfun(External (EF_runtime "__i64_stod"
+                   (mksignature (AST.Tlong :: nil) (Some AST.Tfloat)
+                     cc_default)) (Tcons tlong Tnil) tdouble cc_default)) ::
+ (___i64_utod,
+   Gfun(External (EF_runtime "__i64_utod"
+                   (mksignature (AST.Tlong :: nil) (Some AST.Tfloat)
+                     cc_default)) (Tcons tulong Tnil) tdouble cc_default)) ::
+ (___i64_stof,
+   Gfun(External (EF_runtime "__i64_stof"
+                   (mksignature (AST.Tlong :: nil) (Some AST.Tsingle)
+                     cc_default)) (Tcons tlong Tnil) tfloat cc_default)) ::
+ (___i64_utof,
+   Gfun(External (EF_runtime "__i64_utof"
+                   (mksignature (AST.Tlong :: nil) (Some AST.Tsingle)
+                     cc_default)) (Tcons tulong Tnil) tfloat cc_default)) ::
+ (___i64_sdiv,
+   Gfun(External (EF_runtime "__i64_sdiv"
+                   (mksignature (AST.Tlong :: AST.Tlong :: nil)
+                     (Some AST.Tlong) cc_default))
+     (Tcons tlong (Tcons tlong Tnil)) tlong cc_default)) ::
+ (___i64_udiv,
+   Gfun(External (EF_runtime "__i64_udiv"
+                   (mksignature (AST.Tlong :: AST.Tlong :: nil)
+                     (Some AST.Tlong) cc_default))
+     (Tcons tulong (Tcons tulong Tnil)) tulong cc_default)) ::
+ (___i64_smod,
+   Gfun(External (EF_runtime "__i64_smod"
+                   (mksignature (AST.Tlong :: AST.Tlong :: nil)
+                     (Some AST.Tlong) cc_default))
+     (Tcons tlong (Tcons tlong Tnil)) tlong cc_default)) ::
+ (___i64_umod,
+   Gfun(External (EF_runtime "__i64_umod"
+                   (mksignature (AST.Tlong :: AST.Tlong :: nil)
+                     (Some AST.Tlong) cc_default))
+     (Tcons tulong (Tcons tulong Tnil)) tulong cc_default)) ::
+ (___i64_shl,
+   Gfun(External (EF_runtime "__i64_shl"
+                   (mksignature (AST.Tlong :: AST.Tint :: nil)
+                     (Some AST.Tlong) cc_default))
+     (Tcons tlong (Tcons tint Tnil)) tlong cc_default)) ::
+ (___i64_shr,
+   Gfun(External (EF_runtime "__i64_shr"
+                   (mksignature (AST.Tlong :: AST.Tint :: nil)
+                     (Some AST.Tlong) cc_default))
+     (Tcons tulong (Tcons tint Tnil)) tulong cc_default)) ::
+ (___i64_sar,
+   Gfun(External (EF_runtime "__i64_sar"
+                   (mksignature (AST.Tlong :: AST.Tint :: nil)
+                     (Some AST.Tlong) cc_default))
+     (Tcons tlong (Tcons tint Tnil)) tlong cc_default)) ::
+ (___builtin_bswap,
+   Gfun(External (EF_builtin "__builtin_bswap"
+                   (mksignature (AST.Tint :: nil) (Some AST.Tint) cc_default))
+     (Tcons tuint Tnil) tuint cc_default)) ::
+ (___builtin_bswap32,
+   Gfun(External (EF_builtin "__builtin_bswap32"
+                   (mksignature (AST.Tint :: nil) (Some AST.Tint) cc_default))
+     (Tcons tuint Tnil) tuint cc_default)) ::
+ (___builtin_bswap16,
+   Gfun(External (EF_builtin "__builtin_bswap16"
+                   (mksignature (AST.Tint :: nil) (Some AST.Tint) cc_default))
+     (Tcons tushort Tnil) tushort cc_default)) ::
+ (___builtin_clz,
+   Gfun(External (EF_builtin "__builtin_clz"
+                   (mksignature (AST.Tint :: nil) (Some AST.Tint) cc_default))
+     (Tcons tuint Tnil) tint cc_default)) ::
+ (___builtin_clzl,
+   Gfun(External (EF_builtin "__builtin_clzl"
+                   (mksignature (AST.Tint :: nil) (Some AST.Tint) cc_default))
+     (Tcons tuint Tnil) tint cc_default)) ::
+ (___builtin_clzll,
+   Gfun(External (EF_builtin "__builtin_clzll"
+                   (mksignature (AST.Tlong :: nil) (Some AST.Tint)
+                     cc_default)) (Tcons tulong Tnil) tint cc_default)) ::
+ (___builtin_ctz,
+   Gfun(External (EF_builtin "__builtin_ctz"
+                   (mksignature (AST.Tint :: nil) (Some AST.Tint) cc_default))
+     (Tcons tuint Tnil) tint cc_default)) ::
+ (___builtin_ctzl,
+   Gfun(External (EF_builtin "__builtin_ctzl"
+                   (mksignature (AST.Tint :: nil) (Some AST.Tint) cc_default))
+     (Tcons tuint Tnil) tint cc_default)) ::
+ (___builtin_ctzll,
+   Gfun(External (EF_builtin "__builtin_ctzll"
+                   (mksignature (AST.Tlong :: nil) (Some AST.Tint)
+                     cc_default)) (Tcons tulong Tnil) tint cc_default)) ::
+ (___builtin_fsqrt,
+   Gfun(External (EF_builtin "__builtin_fsqrt"
+                   (mksignature (AST.Tfloat :: nil) (Some AST.Tfloat)
+                     cc_default)) (Tcons tdouble Tnil) tdouble cc_default)) ::
+ (___builtin_fmax,
+   Gfun(External (EF_builtin "__builtin_fmax"
+                   (mksignature (AST.Tfloat :: AST.Tfloat :: nil)
+                     (Some AST.Tfloat) cc_default))
+     (Tcons tdouble (Tcons tdouble Tnil)) tdouble cc_default)) ::
+ (___builtin_fmin,
+   Gfun(External (EF_builtin "__builtin_fmin"
+                   (mksignature (AST.Tfloat :: AST.Tfloat :: nil)
+                     (Some AST.Tfloat) cc_default))
+     (Tcons tdouble (Tcons tdouble Tnil)) tdouble cc_default)) ::
+ (___builtin_fmadd,
+   Gfun(External (EF_builtin "__builtin_fmadd"
+                   (mksignature
+                     (AST.Tfloat :: AST.Tfloat :: AST.Tfloat :: nil)
+                     (Some AST.Tfloat) cc_default))
+     (Tcons tdouble (Tcons tdouble (Tcons tdouble Tnil))) tdouble
+     cc_default)) ::
+ (___builtin_fmsub,
+   Gfun(External (EF_builtin "__builtin_fmsub"
+                   (mksignature
+                     (AST.Tfloat :: AST.Tfloat :: AST.Tfloat :: nil)
+                     (Some AST.Tfloat) cc_default))
+     (Tcons tdouble (Tcons tdouble (Tcons tdouble Tnil))) tdouble
+     cc_default)) ::
+ (___builtin_fnmadd,
+   Gfun(External (EF_builtin "__builtin_fnmadd"
+                   (mksignature
+                     (AST.Tfloat :: AST.Tfloat :: AST.Tfloat :: nil)
+                     (Some AST.Tfloat) cc_default))
+     (Tcons tdouble (Tcons tdouble (Tcons tdouble Tnil))) tdouble
+     cc_default)) ::
+ (___builtin_fnmsub,
+   Gfun(External (EF_builtin "__builtin_fnmsub"
+                   (mksignature
+                     (AST.Tfloat :: AST.Tfloat :: AST.Tfloat :: nil)
+                     (Some AST.Tfloat) cc_default))
+     (Tcons tdouble (Tcons tdouble (Tcons tdouble Tnil))) tdouble
+     cc_default)) ::
+ (___builtin_read16_reversed,
+   Gfun(External (EF_builtin "__builtin_read16_reversed"
+                   (mksignature (AST.Tint :: nil) (Some AST.Tint) cc_default))
+     (Tcons (tptr tushort) Tnil) tushort cc_default)) ::
+ (___builtin_read32_reversed,
+   Gfun(External (EF_builtin "__builtin_read32_reversed"
+                   (mksignature (AST.Tint :: nil) (Some AST.Tint) cc_default))
+     (Tcons (tptr tuint) Tnil) tuint cc_default)) ::
+ (___builtin_write16_reversed,
+   Gfun(External (EF_builtin "__builtin_write16_reversed"
+                   (mksignature (AST.Tint :: AST.Tint :: nil) None
+                     cc_default)) (Tcons (tptr tushort) (Tcons tushort Tnil))
+     tvoid cc_default)) ::
+ (___builtin_write32_reversed,
+   Gfun(External (EF_builtin "__builtin_write32_reversed"
+                   (mksignature (AST.Tint :: AST.Tint :: nil) None
+                     cc_default)) (Tcons (tptr tuint) (Tcons tuint Tnil))
+     tvoid cc_default)) ::
+ (___builtin_nop,
+   Gfun(External (EF_builtin "__builtin_nop"
+                   (mksignature nil None cc_default)) Tnil tvoid cc_default)) ::
+ (___builtin_debug,
+   Gfun(External (EF_external "__builtin_debug"
+                   (mksignature (AST.Tint :: nil) None
+                     {|cc_vararg:=true; cc_unproto:=false; cc_structret:=false|}))
+     (Tcons tint Tnil) tvoid
+     {|cc_vararg:=true; cc_unproto:=false; cc_structret:=false|})) ::
+ (_makelock,
+   Gfun(External (EF_external "makelock"
+                   (mksignature (AST.Tint :: nil) None cc_default))
+     (Tcons (tptr (Tstruct _lock_t noattr)) Tnil) tvoid cc_default)) ::
+ (_freelock,
+   Gfun(External (EF_external "freelock"
+                   (mksignature (AST.Tint :: nil) None cc_default))
+     (Tcons (tptr (Tstruct _lock_t noattr)) Tnil) tvoid cc_default)) ::
+ (_freelock2,
+   Gfun(External (EF_external "freelock2"
+                   (mksignature (AST.Tint :: nil) None cc_default))
+     (Tcons (tptr (Tstruct _lock_t noattr)) Tnil) tvoid cc_default)) ::
+ (_acquire,
+   Gfun(External (EF_external "acquire"
+                   (mksignature (AST.Tint :: nil) None cc_default))
+     (Tcons (tptr (Tstruct _lock_t noattr)) Tnil) tvoid cc_default)) ::
+ (_release,
+   Gfun(External (EF_external "release"
+                   (mksignature (AST.Tint :: nil) None cc_default))
+     (Tcons (tptr (Tstruct _lock_t noattr)) Tnil) tvoid cc_default)) ::
+ (_release2,
+   Gfun(External (EF_external "release2"
+                   (mksignature (AST.Tint :: nil) None cc_default))
+     (Tcons (tptr (Tstruct _lock_t noattr)) Tnil) tvoid cc_default)) ::
+ (_spawn_thread,
+   Gfun(External (EF_external "spawn_thread"
+                   (mksignature (AST.Tint :: AST.Tint :: nil) None
+                     cc_default))
+     (Tcons
+       (tptr (Tfunction (Tcons (tptr tvoid) Tnil) (tptr tvoid) cc_default))
+       (Tcons (tptr tvoid) Tnil)) tvoid cc_default)) ::
+ (_makecond,
+   Gfun(External (EF_external "makecond"
+                   (mksignature (AST.Tint :: nil) None cc_default))
+     (Tcons (tptr tint) Tnil) tvoid cc_default)) ::
+ (_freecond,
+   Gfun(External (EF_external "freecond"
+                   (mksignature (AST.Tint :: nil) None cc_default))
+     (Tcons (tptr tint) Tnil) tvoid cc_default)) ::
+ (_wait,
+   Gfun(External (EF_external "wait"
+                   (mksignature (AST.Tint :: AST.Tint :: nil) None
+                     cc_default))
+     (Tcons (tptr tint) (Tcons (tptr (Tstruct _lock_t noattr)) Tnil)) tvoid
+     cc_default)) ::
+ (_signal,
+   Gfun(External (EF_external "signal"
+                   (mksignature (AST.Tint :: nil) None cc_default))
+     (Tcons (tptr tint) Tnil) tvoid cc_default)) :: (_mutex, Gvar v_mutex) ::
+ (_tlock, Gvar v_tlock) :: (_cond, Gvar v_cond) :: (_data, Gvar v_data) ::
+ (_thread_func, Gfun(Internal f_thread_func)) ::
+ (_main, Gfun(Internal f_main)) :: nil);
+prog_public :=
+(_main :: _thread_func :: _data :: _cond :: _tlock :: _mutex :: _signal ::
+ _wait :: _freecond :: _makecond :: _spawn_thread :: _release2 :: _release ::
+ _acquire :: _freelock2 :: _freelock :: _makelock :: ___builtin_debug ::
+ ___builtin_nop :: ___builtin_write32_reversed ::
+ ___builtin_write16_reversed :: ___builtin_read32_reversed ::
+ ___builtin_read16_reversed :: ___builtin_fnmsub :: ___builtin_fnmadd ::
+ ___builtin_fmsub :: ___builtin_fmadd :: ___builtin_fmin ::
+ ___builtin_fmax :: ___builtin_fsqrt :: ___builtin_ctzll ::
+ ___builtin_ctzl :: ___builtin_ctz :: ___builtin_clzll :: ___builtin_clzl ::
+ ___builtin_clz :: ___builtin_bswap16 :: ___builtin_bswap32 ::
+ ___builtin_bswap :: ___i64_sar :: ___i64_shr :: ___i64_shl :: ___i64_umod ::
+ ___i64_smod :: ___i64_udiv :: ___i64_sdiv :: ___i64_utof :: ___i64_stof ::
+ ___i64_utod :: ___i64_stod :: ___i64_dtou :: ___i64_dtos ::
+ ___compcert_va_composite :: ___compcert_va_float64 ::
+ ___compcert_va_int64 :: ___compcert_va_int32 :: ___builtin_va_end ::
+ ___builtin_va_copy :: ___builtin_va_arg :: ___builtin_va_start ::
+ ___builtin_membar :: ___builtin_annot_intval :: ___builtin_annot ::
+ ___builtin_memcpy_aligned :: ___builtin_fabs :: nil);
+prog_main := _main;
+prog_types := composites;
+prog_comp_env := make_composite_env composites;
+prog_comp_env_eq := refl_equal _
+|}.
+
