progs/verif_cond.v
@@ -1,0 +1,364 @@
+Require Import progs.verif_incr.
+Require Import msl.predicates_sl.
+Require Import floyd.proofauto.
+Require Import concurrency.semax_conc.
+Require Import progs.cond.
+
+Instance CompSpecs : compspecs. make_compspecs prog. Defined.
+Definition Vprog : varspecs. mk_varspecs prog. Defined.
+
+Definition acquire_spec := DECLARE _acquire acquire_spec.
+Definition release_spec := DECLARE _release release_spec.
+Definition makelock_spec := DECLARE _makelock (makelock_spec _).
+Definition freelock_spec := DECLARE _freelock (freelock_spec _).
+Definition spawn_spec := DECLARE _spawn_thread spawn_spec.
+
+Definition freelock2_spec :=
+  DECLARE _freelock2
+   WITH v : val, R : Pred
+   PRE [ _lock OF tptr tlock ]
+     PROP (positive_mpred (Interp R); rec_inv v R)
+     LOCAL (temp _lock v)  
+     SEP (lock_inv Ews v (Interp R))
+   POST [ tvoid ]
+     PROP ()
+     LOCAL ()
+     SEP (data_at_ Ews tlock v).
+
+Definition release2_spec :=
+  DECLARE _release2
+   WITH v : val, sh : share, R : Pred
+   PRE [ _lock OF tptr tlock ]
+     PROP (readable_share sh; precise (Interp R); positive_mpred (Interp R); rec_inv v R)
+     LOCAL (temp _lock v)
+     SEP (Interp R)
+   POST [ tvoid ]
+     PROP ()
+     LOCAL ()
+     SEP (emp).
+
+Definition makecond_spec :=
+  DECLARE _makecond
+   WITH v : val, sh : share
+   PRE [ _cond OF tptr tcond ]
+     PROP (writable_share sh)
+     LOCAL (temp _cond v)
+     SEP (data_at_ sh tcond v)
+   POST [ tvoid ]
+     PROP ()
+     LOCAL ()
+     SEP (cond_var sh v).
+
+Definition freecond_spec :=
+  DECLARE _freecond
+   WITH v : val, sh : share
+   PRE [ _cond OF tptr tcond ]
+     PROP (writable_share sh)
+     LOCAL (temp _cond v)
+     SEP (cond_var sh v)
+   POST [ tvoid ]
+     PROP ()
+     LOCAL ()
+     SEP (data_at_ sh tcond v).
+
+Definition wait_spec :=
+  DECLARE _wait
+   WITH c : val, l : val, shc : share, shl : share, R : Pred
+   PRE [ _cond OF tptr tcond, _mutex OF tptr tlock ]
+     PROP (readable_share shc)
+     LOCAL (temp _cond c; temp _mutex l)
+     SEP (cond_var shc c; lock_inv shl l (Interp R); Interp R)
+   POST [ tvoid ]
+     PROP ()
+     LOCAL ()
+     SEP (cond_var shc c; lock_inv shl l (Interp R); Interp R).
+
+Definition signal_spec :=
+  DECLARE _signal
+   WITH c : val, shc : share
+   PRE [ _cond OF tptr tcond ]
+     PROP (readable_share shc)
+     LOCAL (temp _cond c)
+     SEP (cond_var shc c)
+   POST [ tvoid ]
+     PROP ()
+     LOCAL ()
+     SEP (cond_var shc c).
+
+Definition lock_pred data :=
+  Exp _ (fun i => Data_at _ Ews (tarray tint 1) [Vint (Int.repr i)] data).
+
+Definition tlock_pred sh lockt lock cond data :=
+  Self_lock (Pred_list [Cond_var _ sh cond; Lock_inv sh lock (lock_pred data)]) sh lockt.
+
+Definition thread_func_spec :=
+ DECLARE _thread_func
+  WITH y : val, x : val * share * val * val * val
+  PRE [ _args OF (tptr tvoid) ]
+         let '(data, sh, lock, lockt, cond) := x in
+         PROP  (readable_share sh)
+         LOCAL (temp _args y; gvar _data data; gvar _mutex lock; gvar _tlock lockt;
+                gvar _cond cond)
+         SEP   (cond_var sh cond; lock_inv sh lock (Interp (lock_pred data));
+                lock_inv sh lockt (Interp (tlock_pred sh lockt lock cond data)))
+  POST [ tvoid ]
+         PROP ()
+         LOCAL ()
+         SEP (emp).
+
+Definition main_spec :=
+ DECLARE _main
+  WITH u : unit
+  PRE  [] main_pre prog u
+  POST [ tint ] main_post prog u.
+
+Definition Gprog : funspecs := augment_funspecs prog [acquire_spec; release_spec; release2_spec; makelock_spec;
+  freelock_spec; freelock2_spec; spawn_spec; makecond_spec; freecond_spec; wait_spec; signal_spec;
+  thread_func_spec; main_spec].
+
+Lemma data_at_precise : forall b o,
+  precise (data_at_ Ews (tarray tint 1) (Vptr b o)).
+Proof.
+  intros; unfold data_at_, field_at_, field_at, at_offset; simpl.
+  apply precise_andp2.
+  rewrite data_at_rec_eq; unfold withspacer, at_offset; simpl.
+  unfold array_pred, aggregate_pred.array_pred; simpl.
+  unfold Zlength, Znth; simpl.
+  apply precise_andp2.
+  rewrite data_at_rec_eq; simpl.
+  apply precise_sepcon; [apply mapsto_undef_precise | apply precise_emp]; auto.
+Qed.
+
+Lemma inv_precise : forall b o,
+  precise (EX x : Z, data_at Ews (tarray tint 1) [Vint (Int.repr x)] (Vptr b o)).
+Proof.
+  intros; apply derives_precise with (Q := data_at_ Ews (tarray tint 1) (Vptr b o));
+    [|apply data_at_precise].
+  intros ? (? & ?).
+  apply (data_at_data_at_ _ _ _ _ _ H).
+Qed.
+
+Lemma inv_positive : forall ctr,
+  positive_mpred (EX x : Z, data_at Ews (tarray tint 1) [Vint (Int.repr x)] ctr).
+Proof.
+Admitted.
+
+Lemma cond_var_precise : forall sh b o, readable_share sh ->
+  precise (cond_var sh (Vptr b o)).
+Proof.
+  intros; unfold cond_var, data_at_, field_at_, field_at, at_offset; simpl.
+  apply precise_andp2.
+  rewrite data_at_rec_eq; simpl.
+  apply mapsto_undef_precise; auto.
+Qed.
+
+Lemma positive_sepcon2 : forall P Q (HQ : positive_mpred Q),
+  positive_mpred (P * Q).
+Proof.
+  repeat intro.
+  destruct H as (? & ? & ? & ? & HQ1).
+  specialize (HQ _ HQ1).
+  destruct HQ as (l & sh & rsh & k & p & HQ); exists l, sh, rsh, k, p.
+  admit.
+Admitted.
+
+Lemma cond_var_isptr : forall sh v, cond_var sh v = !! isptr v && cond_var sh v.
+Proof.
+  intros; apply data_at__isptr.
+Qed.
+
+Lemma body_thread_func : semax_body Vprog Gprog f_thread_func thread_func_spec.
+Proof.
+  start_function.
+  forward.
+  forward.
+  forward.
+  forward_call (lock, sh, lock_pred data).
+  simpl.
+  Intro i.
+  forward.
+  forward_call (cond, sh).
+  rewrite field_at_isptr; normalize.
+  forward_call (lock, sh, lock_pred data).
+  { simpl; entailer!.
+    Exists 1.
+    unfold data_at_, field_at_; entailer!. }
+  { split; auto; destruct data; try contradiction; split.
+    - apply inv_precise.
+    - apply inv_positive. }
+  rewrite cond_var_isptr; normalize.
+  forward_call (lockt, sh, tlock_pred sh lockt lock cond data).
+  { subst Frame; instantiate (1 := []); simpl.
+    setoid_rewrite selflock_eq at 2; entailer!.
+    apply lock_inv_later. }
+  { split; auto; simpl; split; [|split]; normalize.
+    - apply selflock_precise, precise_sepcon; [|apply lock_inv_precise].
+      destruct cond; try contradiction; apply cond_var_precise; auto.
+    - apply selflock_positive, positive_sepcon2, lock_inv_positive.
+    - apply selflock_rec. }
+  forward.
+Qed.
+
+Lemma cond_var_almost_empty : forall sh v phi, predicates_hered.app_pred (cond_var sh v) phi ->
+  juicy_machine.almost_empty phi.
+Proof.
+  admit.
+Admitted.
+
+Lemma cond_var_join : forall sh1 sh2 sh v (Hjoin : sepalg.join sh1 sh2 sh),
+  cond_var sh1 v * cond_var sh2 v = cond_var sh v.
+Proof.
+  intros; unfold cond_var; apply data_at__share_join; auto.
+Qed.
+
+Lemma body_main:  semax_body Vprog Gprog f_main main_spec.
+Proof.
+  start_function.
+  rewrite <- (sepcon_emp (main_pre _ _)).
+  rewrite main_pre_start; unfold prog_vars, prog_vars'; simpl globvars2pred.
+  process_idstar.
+  simpl init_data2pred'.
+  rewrite <- (sepcon_emp (_ * _)).
+  simple apply move_globfield_into_SEP.
+  rewrite sepcon_emp.
+  process_idstar.
+  simpl init_data2pred'.
+  rewrite <- (sepcon_emp (_ * _)).
+  simple apply move_globfield_into_SEP.
+  rewrite sepcon_emp.
+  process_idstar.
+  simpl init_data2pred'.
+  rewrite <- (sepcon_emp (_ * _)).
+  simple apply move_globfield_into_SEP.
+  rewrite sepcon_emp.
+  process_idstar.
+  simpl init_data2pred'.
+  rewrite <- (sepcon_emp (_ * _)).
+  simple apply move_globfield_into_SEP.
+  change (globvars2pred nil) with (@emp (environ->mpred) _ _).
+  repeat rewrite sepcon_emp.
+  forward.
+  unfold default_val, upd_Znth, Zlength; simpl.
+  rewrite sublist.sublist_nil.
+  forward.
+  forward.
+  forward.
+  forward_call (gvar2, Ews).
+  { unfold tcond; entailer!. }
+  rewrite field_at_isptr; normalize.
+  destruct split_Ews as (sh1 & sh2 & ? & ? & Hsh).
+  forward_call (gvar0, Ews, lock_pred gvar3).
+  { unfold tlock, semax_conc._lock_t; entailer!. }
+  forward_call (gvar1, Ews, tlock_pred sh1 gvar1 gvar0 gvar2 gvar3).
+  { unfold tlock, semax_conc._lock_t; entailer!. }
+  get_global_function'' _thread_func.
+  normalize.
+  apply extract_exists_pre; intros f_.
+  forward_call (f_, Vint (Int.repr 0), existT (fun ty => ty * (ty -> val -> Pred))%type
+   (val * share * val * val * val)%type ((gvar3, sh1, gvar0, gvar1, gvar2),
+   fun (x : (val * share * val * val * val)) (_ : val) => let '(data, sh, lock, lockt, cond) := x in
+     Pred_list [Pred_prop (readable_share sh); Cond_var _ sh cond; Lock_inv sh lock (lock_pred data);
+                Lock_inv sh lockt (tlock_pred sh lockt lock cond data)])).
+  { entailer.
+    Exists _args; entailer.
+    Exists ([(_data, gvar3); (_mutex, gvar0); (_tlock, gvar1); (_cond, gvar2)]); entailer.
+    subst Frame; instantiate (1 := [lock_inv sh2 gvar1 (Interp (tlock_pred sh1 gvar1 gvar0 gvar2 gvar3));
+      lock_inv sh2 gvar0 (Interp (lock_pred gvar3)); cond_var sh2 gvar2;
+      field_at Ews (tarray tint 1) [] [Vint (Int.repr 0)] gvar3]).
+    simpl; entailer; cancel.
+    repeat rewrite sepcon_assoc.
+    rewrite <- (sepcon_assoc (lock_inv sh1 gvar1 _)).
+    erewrite lock_inv_join; eauto; cancel.
+    repeat rewrite sepcon_assoc.
+    rewrite <- (sepcon_assoc (lock_inv sh1 gvar0 _)).
+    erewrite lock_inv_join; eauto; cancel.
+    rewrite sepcon_assoc; erewrite cond_var_join; eauto; cancel.
+    admit. (* Can we move derives inside func_ptr? Either way, the shape of spawn_spec is unuseful. *) }
+  { simpl; intros ? Hpred.
+    destruct Hpred as (? & ? & ? & ? & ? & ? & ? & ? & ? & ? & ? & ? & ? & ? & ? & ? & Hemp).
+    eapply almost_empty_join; eauto; [|eapply almost_empty_join; eauto;
+      [|eapply almost_empty_join; eauto; [|eapply almost_empty_join; eauto]]].
+    - eapply prop_almost_empty; eauto.
+    - eapply cond_var_almost_empty; eauto.
+    - eapply lock_inv_almost_empty; eauto.
+    - eapply lock_inv_almost_empty; eauto.
+    - eapply emp_almost_empty; eauto. }
+  forward.
+  forward_while (EX i : Z, PROP ( )
+   LOCAL (temp _v (Vint (Int.repr i)); temp _c gvar2; temp _t gvar1; temp _l gvar0; gvar _data gvar3;
+     gvar _cond gvar2; gvar _tlock gvar1; gvar _mutex gvar0)
+   SEP (lock_inv sh2 gvar1 (Interp (tlock_pred sh1 gvar1 gvar0 gvar2 gvar3));
+        lock_inv sh2 gvar0 (Interp (lock_pred gvar3)); cond_var sh2 gvar2;
+        Interp (lock_pred gvar3))).
+  { Exists 0; entailer!.
+    Exists 0; entailer. }
+  { entailer. }
+  - (* loop body *)
+    forward_call (gvar2, gvar0, sh2, sh2, lock_pred gvar3).
+    simpl; Intro i'.
+    forward.
+    Exists i'; entailer.
+    Exists i'; entailer!.
+  - forward_call (gvar1, sh2, tlock_pred sh1 gvar1 gvar0 gvar2 gvar3).
+    forward_call (gvar1, Later (tlock_pred sh1 gvar1 gvar0 gvar2 gvar3)).
+    { subst Frame; instantiate (1 := [lock_inv Ews gvar0 (Interp (lock_pred gvar3));
+        cond_var Ews gvar2; Interp (lock_pred gvar3)]); simpl; cancel.
+      rewrite selflock_eq at 2.
+      rewrite sepcon_assoc, <- (sepcon_assoc (lock_inv _ gvar1 _)), (sepcon_comm (lock_inv _ gvar1 _)).
+      repeat rewrite sepcon_assoc; rewrite <- (sepcon_assoc (lock_inv sh2 gvar1 _)).
+      apply sepalg.join_comm in Hsh.
+      eapply derives_trans.
+      { apply sepcon_derives; [apply derives_refl|].
+        apply sepcon_derives; [apply derives_refl|].
+        apply sepcon_derives; [|apply derives_refl].
+        apply sepcon_derives; [apply lock_inv_later | apply derives_refl]. }
+      erewrite lock_inv_join; eauto; cancel.
+      repeat rewrite sepcon_assoc; rewrite <- (sepcon_assoc (lock_inv _ gvar0 _)).
+      apply sepalg.join_comm in Hsh.
+      erewrite lock_inv_join; eauto; cancel.
+      erewrite cond_var_join; eauto. }
+    { split.
+      + apply later_positive, selflock_positive; simpl.
+        apply positive_sepcon2, positive_sepcon1, lock_inv_positive.
+      + apply later_rec, selflock_rec. }
+    forward_call (gvar0, Ews, lock_pred gvar3).
+    { split; [auto | apply inv_positive]. }
+    forward_call (gvar2, Ews).
+    forward.
+Admitted.
+
+Definition extlink := ext_link_prog prog.
+
+Definition Espec := add_funspecs (Concurrent_Espec unit _ extlink) extlink Gprog.
+Existing Instance Espec.
+
+Lemma all_funcs_correct:
+  semax_func Vprog Gprog (prog_funct prog) Gprog.
+Proof.
+unfold Gprog, prog, prog_funct; simpl.
+repeat (apply semax_func_cons_ext_vacuous; [reflexivity | ]).
+semax_func_cons_ext.
+{ admit. }
+semax_func_cons_ext.
+{ admit. }
+semax_func_cons_ext.
+{ admit. }
+semax_func_cons_ext.
+{ admit. }
+semax_func_cons_ext.
+{ admit. }
+semax_func_cons_ext.
+{ admit. }
+semax_func_cons_ext.
+{ admit. }
+semax_func_cons_ext.
+{ admit. }
+semax_func_cons_ext.
+{ admit. }
+semax_func_cons_ext.
+{ admit. }
+semax_func_cons_ext.
+{ admit. }
+semax_func_cons body_thread_func.
+semax_func_cons body_main.
+Admitted.
